packet.v
@@ -1,14 +1,202 @@
 Require Import ZArith.
 
-Inductive packet_type : Set := RRQ | WRQ | DATA | ACK | ERROR.
 
-Definition type_to_int (type: packet_type) : positive :=
-  match type with  
-    | RRQ   => 1
-    | WRQ   => 2
-    | DATA  => 3
-    | ACK   => 4
-    | ERROR => 5
+Local Open Scope positive_scope.
+
+Unset Elimination Schemes.
+Inductive packet_opcode : Set := RRQ | WRQ | DATA | ACK | ERROR.
+
+Definition opcode_to_nr (code: packet_opcode) :=
+  match code with  
+  | RRQ   => 1
+  | WRQ   => 2
+  | DATA  => 3
+  | ACK   => 4
+  | ERROR => 5
+  end.
+
+Lemma opcode_range : forall x, 1 <= opcode_to_nr x <= 5.
+Proof.
+intros.
+destruct x.
+all: easy.
+Qed.
+
+
+Definition nr_to_opcode (nr: positive) : option packet_opcode := 
+  match nr with
+  | 1 => Some RRQ
+  | 2 => Some WRQ
+  | 3 => Some DATA
+  | 4 => Some ACK
+  | 5 => Some ERROR
+  | _ => None
   end.
 
 
+Lemma nr_opcode_ident : forall x, (x = 1 \/ x = 2 \/ x = 3 \/ x = 4 \/ x = 5) ->
+  match nr_to_opcode x with 
+    | Some opcode => x = opcode_to_nr opcode
+    | None => True
+  end.
+Proof.
+intros x bounds.
+case bounds.
+* intros.
+  rewrite H.
+  unfold nr_to_opcode.
+  auto.
+* intros bounds2.
+  case bounds2.
+  + intros.
+    rewrite H.
+    unfold nr_to_opcode.
+    auto.
+  + intros bounds3.
+    case bounds3.
+    - intros.
+      rewrite H.
+      unfold nr_to_opcode.
+      auto.
+    - intros bounds4.
+      case bounds4.
+      all: intros.
+      all: rewrite H.
+      all: unfold nr_to_opcode.
+      all: auto.
+Qed.
+
+
+Lemma nr_opcode_none : forall x, x > 5 \/ x < 1 -> nr_to_opcode x = None.
+Proof.
+intros.
+unfold nr_to_opcode.
+case H.
+* intro gt5.
+  destruct x.
+  + destruct x.
+    - trivial.
+    - destruct x; easy.
+    - easy.
+  + destruct x.
+    - trivial.
+    - destruct x; easy.
+    - easy.
+  + easy.
+* intro.
+  destruct x.  
+  all: easy.
+Qed.
+
+Require Import Ascii.
+
+Open Scope char_scope.
+
+Definition opcode_to_ascii (op : packet_opcode) : ascii :=
+   ascii_of_pos (opcode_to_nr op).
+
+Theorem opcode_to_ascii_and_back : forall op : packet_opcode, N_of_ascii (opcode_to_ascii op) = Npos (opcode_to_nr op).
+Proof.
+intros.
+destruct op.
+all: simpl.
+all: trivial.
+Qed.
+
+(* FMLLLLL
+      all: auto.
+      exfalso.
+      assert (5 < 4).
+      { apply Pos.gt_lt_iff. assumption. }
+      assert (2 < 1).
+      { apply Pos.succ_lt_mono. apply Pos.succ_lt_mono. apply Pos.succ_lt_mono. assumption. }
+      apply (Pos.nlt_1_r 2).
+      assumption.
+    - exfalso.
+      easy.
+      assert (5 < 2).
+      { apply Pos.gt_lt_iff. assumption. }
+      assert (4 < 1).
+      { apply Pos.succ_lt_mono. assumption. }
+      apply (Pos.nlt_1_r 4).
+      assumption.
+  + exfalso.
+    cut (5 < 1).
+    ** intros.
+       apply (Pos.nlt_1_r 5).
+       assumption.
+    ** apply Pos.gt_lt_iff. assumption.
+* intros lt1.
+  exfalso.
+  apply (Pos.nlt_1_r x).
+  assumption.
+Qed.*)
+
+Inductive error_code : Set := 
+| NOT_DEFINED 
+| FILE_NOT_FOUND 
+| ACCESS_VIOLATION
+| DISK_FULL_OR_ALLOCATION_EXCEEDED
+| ILLEGAL_TFTP_OPERATION
+| UNKNOWN_TRANSFER_ID
+| FILE_ALREADY_EXISTS.
+
+
+
+Inductive mode : Set := Read | Write.
+
+
+Require Import String.
+
+Inductive packet : Set := 
+| p_RRQ : string -> packet                  (* Filename *)
+| p_WRQ : string -> packet                  (* Filename *)
+| p_DATA : positive -> string -> packet     (* Block #, Data *)
+| p_ACK : positive -> packet                (* Block # *)
+| p_ERROR : error_code -> string -> packet. (* ErrorCode, ErrMsg *)
+
+
+Definition init_packet (m : mode) (filename : string) : packet := 
+  match m with
+  | Read => p_RRQ filename
+  | Write => p_WRQ filename
+  end.
+
+Theorem init_packet_read_rrq : forall s : string, forall m : mode, m = Read -> init_packet m s = p_RRQ s.
+Proof.
+intros.
+unfold init_packet.
+rewrite H.
+auto.
+Qed.
+
+Theorem init_packet_write_wrq : forall s : string, forall m : mode, m = Write -> init_packet m s = p_WRQ s.
+Proof.
+intros.
+unfold init_packet.
+rewrite H.
+auto.
+Qed.
+
+
+
+
+Definition serialize_packet (p : packet) : string := 
+  match p with
+  | p_RRQ filename => String "000" (String (opcode_to_ascii RRQ) (filename ++ String "000" ("octet" ++ String "000" EmptyString))).
+  | p_WRQ filename => String "000" (String (opcode_to_ascii WRQ) (filename ++ String "000" ("octet" ++ String "000" EmptyString))).
+  | p_DATA 
+
+(* client *)
+
+
+
+Record init_state : Set := mkState {
+    transfer_mode : mode;
+    filename : string;
+    port: positive;
+    last_packet : option packet;
+    timeout_count : N;
+}.
+
+Definition coq_process_state () := .
