extraction.v
@@ -1,0 +1,13 @@
+Require Coq_uniq.
+
+Require Import ExtrOcamlBasic.
+Require Import ExtrOcamlString.
+
+Extraction Blacklist String Int List Nat.
+
+(* tak można wstawiać ocamlowy kod do aksjomatów *)
+Extract Constant Coq_uniq.newline => "'\n'".
+
+Separate Extraction
+         BinNat BinNums BinInt BinPos (* to jest potrzebne do camlcoq *)
+         Coq_uniq.
