Makefile
@@ -1,0 +1,12 @@
+
+coq_grep: extract
+	ocamlbuild uniq.byte
+
+extract: extraction.v Coq_uniq.vo
+	coqtop -batch -load-vernac-source $<
+
+%.vo: %.v
+	coqc $<
+
+clean:
+	rm -f *.o *.cmi *.cmo *.cmx *.vo
